@prefix : <https://w3id.org/fdof/ontology#> .
@prefix dct: <http://purl.org/dc/terms/> .
@prefix mod: <https://w3id.org/mod#> .
@prefix omv: <http://omv.ontoware.org/2005/05/ontology#> .
@prefix owl: <http://www.w3.org/2002/07/owl#> .
@prefix rdf: <http://www.w3.org/1999/02/22-rdf-syntax-ns#> .
@prefix xml: <http://www.w3.org/XML/1998/namespace> .
@prefix xsd: <http://www.w3.org/2001/XMLSchema#> .
@prefix dcat: <http://www.w3.org/ns/dcat#> .
@prefix fdof: <https://w3id.org/fdof/ontology#> .
@prefix gufo: <http://purl.org/nemo/gufo#> .
@prefix meta: <https://w3id.org/fdof/ontology/metadata/> .
@prefix rdfs: <http://www.w3.org/2000/01/rdf-schema#> .
@prefix vann: <http://purl.org/vocab/vann/> .
@base <https://w3id.org/fdof/ontology> .

<https://w3id.org/fdof/ontology> rdf:type owl:Ontology ;
                                  owl:versionIRI <https://w3id/fdof/ontotlogy/1.1.0> ;
                                  owl:imports <http://purl.org/nemo/gufo#/1.0.0> ;
                                  dct:bibliographicCitation "Santos, L. O. B. D. S., Sales, T. P., Fonseca, C. M., & Guizzardi, G. (2023). Towards a conceptual model for the FAIR Digital Object Framework. arXiv preprint arXiv:2302.11894. https://doi.org/10.48550/arXiv.2302.11894"@en ;
                                  dct:creator <https://orcid.org/0000-0002-1164-1351> ,
                                              <https://orcid.org/0000-0002-3452-553X> ,
                                              <https://orcid.org/0000-0002-5385-5761> ,
                                              <https://orcid.org/0000-0003-2528-3118> ;
                                  dct:description "The FAIR Digital Object Framework Ontology (FDOF-O) is an OWL ontology designed to support the semantic annotation of FAIR Information Objects and FAIR Media Objects enabling application-specific requirements."@en ;
                                  dct:issued "2023-02-10"^^xsd:date ;
                                  dct:license <https://creativecommons.org/licenses/by-sa/3.0> ;
                                  dct:publisher <https://www.utwente.nl/eemcs/scs/> ;
                                  dct:title "FDOF-O: FAIR Digital Object Framework Ontology"@en ;
                                  vann:preferredNamespacePrefix "fdof"@en ;
                                  vann:preferredNamespaceUri "https://w3id/fdof/ontotlogy#"^^xsd:anyURI ;
                                  owl:versionInfo "1.1.0"@en ;
                                  dcat:distribution fdof:fdofTtl ;
                                  dcat:landingPage <https://github.com/utwente-scs/fdof-o/> ;
                                  mod:acronym "FDOF-O" ;
                                  mod:hasRepresentationLanguage omv:OWL ;
                                  mod:vocabularyUsed omv: ,
                                                     dct: ,
                                                     gufo: ,
                                                     vann: ,
                                                     rdf: ,
                                                     rdfs: ,
                                                     xsd: ,
                                                     owl: ,
                                                     dcat: ,
                                                     mod: .

#################################################################
#    Annotation properties
#################################################################

###  http://purl.org/dc/terms/bibliographicCitation
dct:bibliographicCitation rdf:type owl:AnnotationProperty .


###  http://purl.org/dc/terms/creator
dct:creator rdf:type owl:AnnotationProperty .


###  http://purl.org/dc/terms/description
dct:description rdf:type owl:AnnotationProperty .


###  http://purl.org/dc/terms/issued
dct:issued rdf:type owl:AnnotationProperty .


###  http://purl.org/dc/terms/license
dct:license rdf:type owl:AnnotationProperty .


###  http://purl.org/dc/terms/publisher
dct:publisher rdf:type owl:AnnotationProperty .


###  http://purl.org/dc/terms/title
dct:title rdf:type owl:AnnotationProperty .


###  http://purl.org/vocab/vann/preferredNamespacePrefix
vann:preferredNamespacePrefix rdf:type owl:AnnotationProperty .


###  http://purl.org/vocab/vann/preferredNamespaceUri
vann:preferredNamespaceUri rdf:type owl:AnnotationProperty .


###  http://www.w3.org/ns/dcat#distribution
dcat:distribution rdf:type owl:AnnotationProperty .


###  http://www.w3.org/ns/dcat#landingPage
dcat:landingPage rdf:type owl:AnnotationProperty .


###  https://w3id.org/mod#acronym
mod:acronym rdf:type owl:AnnotationProperty .


###  https://w3id.org/mod#hasRepresentationLanguage
mod:hasRepresentationLanguage rdf:type owl:AnnotationProperty .


###  https://w3id.org/mod#vocabularyUsed
mod:vocabularyUsed rdf:type owl:AnnotationProperty .


#################################################################
#    Object Properties
#################################################################

###  http://purl.org/nemo/gufo#hasReifiedQualityValue
gufo:hasReifiedQualityValue rdf:type owl:ObjectProperty .


###  http://purl.org/nemo/gufo#historicallyDependsOn
gufo:historicallyDependsOn rdf:type owl:ObjectProperty .


###  https://w3id.org/fdof/ontology#hasEncodingFormat
fdof:hasEncodingFormat rdf:type owl:ObjectProperty ;
                       rdfs:domain fdof:FAIRMediaObject ;
                       dct:description "Identifies the encoding format of the FAIR Media Object in terms of some well-defined media type, such as an IANA media types."@en ;
                       rdfs:label "has encoding format"@en ,
                                  "hasEncodingFormat"@en .


###  https://w3id.org/fdof/ontology#hasInformationObjectType
fdof:hasInformationObjectType rdf:type owl:ObjectProperty ;
                              rdfs:domain fdof:FAIRInformationObject ;
                              rdfs:range fdof:FAIRInformationObjectType ;
                              dct:description "Identifies the FAIR Information Object Type that defines the complaince requirements the FAIR Information Object adheres to in some specific implementation of the FAIR principles."@en ;
                              rdfs:label "has information object type"@en ,
                                         "hasInformationObjectType"@en .


###  https://w3id.org/fdof/ontology#hasMetadata
fdof:hasMetadata rdf:type owl:ObjectProperty ;
                 owl:inverseOf fdof:isMetadataOf ;
                 rdfs:domain fdof:DigitalObject ;
                 rdfs:range fdof:MetadataRecord ;
                 dct:description """Identifies a fdof:MetadataRecord named graph that aggregates all triples of a metadata record of the fdof:DigitalObject.

For example, the named graph meta:fdofMetadata is a fdof:FAIRMetadataRecord about <https://w3id.org/fdof/ontology>."""@en ;
                 rdfs:label "has metadata"@en ,
                            "hasMetadata"@en .


###  https://w3id.org/fdof/ontology#isIdentifiedBy
fdof:isIdentifiedBy rdf:type owl:ObjectProperty ;
                    rdfs:subPropertyOf gufo:hasReifiedQualityValue ;
                    rdfs:range fdof:Identifier ;
                    dct:description """Identifies an identifier of an object reified as a fdof:Identifier

For example,  a hypothetical object <https://w3id.org/fdof/ontology#identifier> that represents an identifier of <https://w3id.org/fdof/ontology>."""@en ;
                    rdfs:label "is identified by"@en ,
                               "isIdentifiedBy"@en .


###  https://w3id.org/fdof/ontology#isMaterializedBy
fdof:isMaterializedBy rdf:type owl:ObjectProperty ;
                      owl:inverseOf fdof:materializes ;
                      rdfs:domain fdof:InformationObject ;
                      rdfs:range fdof:MediaObject ;
                      dct:description """Identifies a fdof:MediaObject that is a materialization of the fdof:InformationObject.

For example, the <https://w3id.org/fdof/ontology> is materialized by fdof:fdofTtl, which is a Turtle file. This is an example of a complete materialization, but partial materializations and equivalent materializations are both allowed."""@en ;
                      rdfs:label "is materialized by"@en ,
                                 "isMaterializedBy"@en .


###  https://w3id.org/fdof/ontology#isMetadataOf
fdof:isMetadataOf rdf:type owl:ObjectProperty ;
                  rdfs:subPropertyOf gufo:historicallyDependsOn ;
                  rdfs:domain fdof:MetadataRecord ;
                  rdfs:range fdof:DigitalObject ;
                  dct:description "Identifies the fdof:DigitalObject the fdof:MetadataRecord is about."@en ;
                  rdfs:label "is metadata of"@en ,
                             "isMetadataOf"@en .


###  https://w3id.org/fdof/ontology#materializes
fdof:materializes rdf:type owl:ObjectProperty ;
                  rdfs:subPropertyOf gufo:historicallyDependsOn ;
                  rdfs:domain fdof:MediaObject ;
                  rdfs:range fdof:InformationObject ;
                  dct:description """Identifies a fdof:InformationObject it materializes. Inverse property of fdof:isMaterializedBy.

Similarly to the materialization of a fdof:InformationObject into one or more fdof:MediaObject, a fdof:MediaObject can also materilize a portion of or several fdof:InformationObject."""@en ;
                  rdfs:label "materializes"@en .


#################################################################
#    Data properties
#################################################################

###  https://w3id.org/fdof/ontology#gupri
fdof:gupri rdf:type owl:DatatypeProperty ;
           rdfs:subPropertyOf fdof:identifier ;
           rdfs:domain fdof:FAIRDigitalObject ;
           dct:description "Determines the globally unique, persistent and resolvable identifier of a FAIR Digital Object in a literal representation."@en ;
           rdfs:label "globally unique, persistent and resolvable identifier"@en ,
                      "gupri"@en .


###  https://w3id.org/fdof/ontology#identifier
fdof:identifier rdf:type owl:DatatypeProperty ;
                rdfs:domain fdof:IdentifiedDigitalObject ;
                dct:description "Determines the identifier of an Identified Digital Object in a literal representation."@en ;
                rdfs:label "identifier"@en .


#################################################################
#    Classes
#################################################################

###  http://purl.org/nemo/gufo#AbstractIndividual
gufo:AbstractIndividual rdf:type owl:Class .


###  http://purl.org/nemo/gufo#AbstractIndividualType
gufo:AbstractIndividualType rdf:type owl:Class .


###  http://purl.org/nemo/gufo#Category
gufo:Category rdf:type owl:Class .


###  http://purl.org/nemo/gufo#Kind
gufo:Kind rdf:type owl:Class .


###  http://purl.org/nemo/gufo#Object
gufo:Object rdf:type owl:Class .


###  http://purl.org/nemo/gufo#Role
gufo:Role rdf:type owl:Class .


###  http://purl.org/nemo/gufo#RoleMixin
gufo:RoleMixin rdf:type owl:Class .


###  http://purl.org/nemo/gufo#SubKind
gufo:SubKind rdf:type owl:Class .


###  https://w3id.org/fdof/ontology#Dataset
fdof:Dataset rdf:type owl:Class ;
             rdfs:subClassOf fdof:InformationObject .


###  https://w3id.org/fdof/ontology#DigitalObject
fdof:DigitalObject rdf:type owl:Class ;
                   rdfs:subClassOf gufo:Object .


###  https://w3id.org/fdof/ontology#FAIRDigitalObject
fdof:FAIRDigitalObject rdf:type owl:Class ;
                       rdfs:subClassOf fdof:IdentifiedDigitalObject .


###  https://w3id.org/fdof/ontology#FAIRInformationObject
fdof:FAIRInformationObject rdf:type owl:Class ;
                           rdfs:subClassOf fdof:FAIRDigitalObject ,
                                           fdof:InformationObject .


###  https://w3id.org/fdof/ontology#FAIRInformationObjectType
fdof:FAIRInformationObjectType rdf:type owl:Class ;
                               rdfs:subClassOf gufo:Type ;
                               dct:description "FAIR Information Object Type is second-order type that defines the requirements of an implementation of the FAIR principles and that are fulfilled by its instances."@en ;
                               rdfs:label "FAIR Information Object Type"@en ,
                                          "FAIRInformationObjectType"@en .


###  https://w3id.org/fdof/ontology#FAIRMediaObject
fdof:FAIRMediaObject rdf:type owl:Class ;
                     rdfs:subClassOf fdof:FAIRDigitalObject ,
                                     fdof:MediaObject .


###  https://w3id.org/fdof/ontology#FAIRMetadataRecord
fdof:FAIRMetadataRecord rdf:type owl:Class ;
                        rdfs:subClassOf fdof:FAIRInformationObject ,
                                        fdof:MetadataRecord .


###  https://w3id.org/fdof/ontology#GUPRI
fdof:GUPRI rdf:type owl:Class ;
           rdfs:subClassOf fdof:Identifier .


###  https://w3id.org/fdof/ontology#IdentifiedDigitalObject
fdof:IdentifiedDigitalObject rdf:type owl:Class ;
                             rdfs:subClassOf fdof:DigitalObject .


###  https://w3id.org/fdof/ontology#Identifier
fdof:Identifier rdf:type owl:Class ;
                rdfs:subClassOf gufo:AbstractIndividual .


###  https://w3id.org/fdof/ontology#InformationObject
fdof:InformationObject rdf:type owl:Class ;
                       rdfs:subClassOf fdof:DigitalObject ,
                                       [ rdf:type owl:Restriction ;
                                         owl:onProperty fdof:isMaterializedBy ;
                                         owl:someValuesFrom fdof:MediaObject
                                       ] ;
                       owl:disjointWith fdof:MediaObject .


###  https://w3id.org/fdof/ontology#MediaObject
fdof:MediaObject rdf:type owl:Class ;
                 rdfs:subClassOf fdof:DigitalObject .


###  https://w3id.org/fdof/ontology#MetadataRecord
fdof:MetadataRecord rdf:type owl:Class ;
                    rdfs:subClassOf fdof:Dataset ,
                                    [ rdf:type owl:Restriction ;
                                      owl:onProperty fdof:isMetadataOf ;
                                      owl:someValuesFrom fdof:DigitalObject
                                    ] .


#################################################################
#    Individuals
#################################################################

###  https://w3id.org/fdof/ontology
<https://w3id.org/fdof/ontology> rdf:type owl:NamedIndividual ,
                                          fdof:FAIRInformationObject ;
                                 fdof:isMaterializedBy fdof:fdofTtl ;
                                 fdof:gupri "https://w3id.org/fdof/ontology"^^xsd:anyURI .


###  https://w3id.org/fdof/ontology#Dataset
fdof:Dataset rdf:type owl:NamedIndividual ,
                      gufo:SubKind .


###  https://w3id.org/fdof/ontology#DigitalObject
fdof:DigitalObject rdf:type owl:NamedIndividual ,
                            gufo:Category .


###  https://w3id.org/fdof/ontology#FAIRDigitalObject
fdof:FAIRDigitalObject rdf:type owl:NamedIndividual ,
                                gufo:RoleMixin .


###  https://w3id.org/fdof/ontology#FAIRInformationObject
fdof:FAIRInformationObject rdf:type owl:NamedIndividual ,
                                    gufo:Role .


###  https://w3id.org/fdof/ontology#FAIRMediaObject
fdof:FAIRMediaObject rdf:type owl:NamedIndividual ,
                              gufo:Role .


###  https://w3id.org/fdof/ontology#FAIRMetadataRecord
fdof:FAIRMetadataRecord rdf:type owl:NamedIndividual ,
                                 gufo:Role .


###  https://w3id.org/fdof/ontology#GUPRI
fdof:GUPRI rdf:type owl:NamedIndividual ,
                    gufo:AbstractIndividualType .


###  https://w3id.org/fdof/ontology#IdentifiedDigitalObject
fdof:IdentifiedDigitalObject rdf:type owl:NamedIndividual ,
                                      gufo:RoleMixin .


###  https://w3id.org/fdof/ontology#Identifier
fdof:Identifier rdf:type owl:NamedIndividual ,
                         gufo:AbstractIndividualType .


###  https://w3id.org/fdof/ontology#InformationObject
fdof:InformationObject rdf:type owl:NamedIndividual ,
                                gufo:Kind .


###  https://w3id.org/fdof/ontology#MediaObject
fdof:MediaObject rdf:type owl:NamedIndividual ,
                          gufo:Kind .


###  https://w3id.org/fdof/ontology#MetadataRecord
fdof:MetadataRecord rdf:type owl:NamedIndividual ,
                             gufo:Role .


###  https://w3id.org/fdof/ontology#fdofTtl
fdof:fdofTtl rdf:type owl:NamedIndividual .


#################################################################
#    Annotations
#################################################################

fdof:Dataset dct:description "Dataset is a type of Information Object designed to collect multiple Data Items"@en ;
             rdfs:label "Dataset"@en .


fdof:DigitalObject rdfs:label "DigitalObject"@en ,
                              "Digital Object"@en ;
                   dct:description """Digital Object is a category of Object characterized for being represented in a digital format.

Examples of Digital objects include media objects (e.g., a digital image) and information object (e.g., an entry on a SQL table)."""@en .


fdof:FAIRDigitalObject dct:description "FAIR Digital Objects represent informational entitied present in digital space that follow the FAIR principles. FAIR Digital Objects must be identified by globally unique, persistent and resolvable identifiers and should be described by rich metadata."@en ;
                       rdfs:label "FAIRDigitalObject"@en ,
                                  "FAIR Digital Object"@en .


fdof:FAIRInformationObject rdfs:label "FAIRInformationObject"@en ;
                           dct:description "FAIR Information Object is a specialised type of FAIR Digital Object that represents units of information. FAIR Information Objects are materialised by at least one FAIR Media Object."@en ;
                           rdfs:label "FAIR Information Object"@en .


fdof:FAIRMediaObject dct:description "FAIR Media Object is a bit sequence which encodes the informational content of at least on FAIR Information Object. FAIR Media Objects serialise characteristics that are proper to its related media encoding type."@en ;
                     rdfs:label "FAIR Media Object"@en ,
                                "FAIRMediaObject"@en .


fdof:FAIRMetadataRecord rdfs:label "FAIRMetadataRecord"@en ,
                                   "FAIR Metadata Record"@en ;
                        dct:description "FAIR Metadata Record is type of FAIR Digital Information Object that collects Date Items about some FAIR Information Object."@en .


fdof:GUPRI dct:description "Globally Unique, Persistent and Resolvable Identifier (GUPRI) specialises the concept of identifier by requiring the identifier to be globally unique, persistent and resolvable as per  FAIR principles F1 and A1."@en ;
           rdfs:label "GUPRI"@en ,
                      "GloballyUnique, Persistent and Resolvable Identifier"@en .


fdof:IdentifiedDigitalObject rdfs:label "IdentifiedDigitalObject"@en ,
                                        "Identified Digital Object"@en ;
                             dct:description "Identified Digital Object is a type of Digital Object that bear an Identifier."@en .


fdof:Identifier rdfs:label "Identifier"@en ;
                dct:description "Identifier is a type of entity that uniquelly identifies an Object with a certain scope."@en .


fdof:InformationObject rdfs:label "InformationObject"@en ;
                       dct:description "Information Object is a type of Object that represents some informational content and is materialized in one or more Media Objects."@en ;
                       rdfs:label "Information Object"@en .


fdof:MediaObject dct:description "Media Object is a type of Object characterized by a certain Encoding Format and that serves as means for the materialization of one or more Information Objects."@en ;
                 rdfs:label "Media Object"@en ,
                            "MediaObject"@en .


fdof:MetadataRecord rdfs:label "Metadata Record"@en ;
                    dct:description "Metadata Record is type of Dataset that collects Date Items about some Object."@en ;
                    rdfs:label "MetadataRecord"@en .


###  Generated by the OWL API (version 4.5.9.2019-02-01T07:24:44Z) https://github.com/owlcs/owlapi
